proofs/Symcrust/Properties/Ntt.lean
@@ -3,6 +3,7 @@ import Symcrust.Properties.BarrettReduction
 import Symcrust.Properties.MontReduction
 import Symcrust.Properties.NttSpecAux
 import Symcrust.Properties.NormMod
+import Symcrust.Properties.Basic
 
 open Aeneas
 open Std
@@ -21,6 +22,7 @@ set_option maxRecDepth 2048
 @[local simp] theorem bv_shift_16_eq_div (x : BitVec 32) : x >>> 16 = x / 65536#32 := by bv_decide
 @[local simp] theorem nat_and_65535_eq_mod (x : Nat) : x &&& 65535 = x % 65536 := by apply Nat.and_two_pow_sub_one_eq_mod x 16
 
+-- TODO: remove those simps
 @[local simp]
 theorem mod_4294967296_65536_eq (x : Nat) : ((x % 4294967296) % 65536) = x % 65536 := by
   rw [Nat.mod_mod_of_dvd]; omega
@@ -53,33 +55,6 @@ bit-vectors.
 attribute [-progress] UScalar.cast.progress_spec
 attribute [local progress] UScalar.cast_inBounds_spec
 
-def to_poly (a : Array U16 256#usize) : Spec.Polynomial := Vector.ofFn (fun i => a[i]!)
-
-@[simp]
-theorem getElem!_to_poly (a : Array U16 256#usize) (i : ℕ) :
-  (to_poly a)[i]! = ((a.val[i]!) : Spec.Zq) := by
-  simp [to_poly]
-  dcases hi : i < a.val.length <;> simp_all [default, Vector.getElem!_ofFn]
-
-@[simp]
-theorem to_poly_set (a : Array U16 256#usize) (i : Usize) (x : U16) :
-  to_poly (Std.Array.set a i x) = (to_poly a).set! i.val (x.val : Spec.Zq) := by
-  simp only [to_poly, Spec.Q, id_eq, Array.set_val_eq, List.map_set]
-  rw [Vector.eq_iff_forall_eq_getElem!]
-  intro j hj
-  simp_lists
-  by_cases hj': j = i <;> simp only [Fin.getElem!_fin, Array.getElem!_Nat_eq, Array.set_val_eq,
-    Nat.not_eq, ne_eq, not_false_eq_true, lt_or_lt_iff_ne, true_or, or_true, List.getElem!_set_ne,
-    id_eq, hj']
-  simp_lists
-  simp_lists -- TODO: why do we need two calls?
-
-@[simp]
-theorem to_poly_getElem!_eq (a : Std.Array U16 256#usize) (i : Nat) :
-  (to_poly a)[i]! = a.val[i]! := by
-  fsimp [to_poly]
-  dcases h: i < 256 <;> simp_all [Vector.getElem!_ofFn, default]
-
 @[local simp]
 theorem Nat_mod_3329_mod_4294967296_eq (x : Nat) :
   x % 3329 % 4294967296 = x % 3329 := by
@@ -91,22 +66,6 @@ theorem Int_mod_3329_mod_4294967296_eq (x : Int) :
   apply Int.emod_eq_of_lt <;> omega
 
 namespace ntt
-
-@[simp, scalar_tac_simps, bvify_simps] theorem Q.eq : Q = 3329#u32 := by simp [global_simps]
-@[simp, scalar_tac_simps, bvify_simps] theorem NEG_Q_INV_MOD_R.eq : NEG_Q_INV_MOD_R = 3327#u32 := by simp [global_simps]
-@[simp, scalar_tac_simps, bvify_simps] theorem RMASK.eq : RMASK = 65535#u32 := by simp [global_simps]
-@[simp, scalar_tac_simps, bvify_simps] theorem RLOG2.eq : RLOG2 = 16#u32 := by simp [global_simps]
-@[simp, scalar_tac_simps, bvify_simps] theorem RSQR.eq : RSQR = 1353#u32 := by simp [global_simps]
-@[simp, scalar_tac_simps, bvify_simps] theorem RSQR_TIMES_NEG_Q_INV_MOD_R.eq : RSQR_TIMES_NEG_Q_INV_MOD_R = 44983#u32 := by simp [global_simps]
-
-@[simp, scalar_tac_simps, bvify_simps]
-theorem key.MLWE_POLYNOMIAL_COEFFICIENTS_eq : key.MLWE_POLYNOMIAL_COEFFICIENTS.val = 256 := by simp [global_simps]
-
-@[simp] theorem INTT_FIXUP_TIMES_RSQR.eq : INTT_FIXUP_TIMES_RSQR.val = 1441 := by simp [global_simps]
-@[simp] theorem INTT_FIXUP_TIMES_RSQR.bv_eq : INTT_FIXUP_TIMES_RSQR.bv = 1441#32 := by simp [global_simps]
-
-@[simp] theorem INTT_FIXUP_TIMES_RSQR_TIMES_NEQ_Q_INV_MOD_R.bv_eq : INTT_FIXUP_TIMES_RSQR_TIMES_NEQ_Q_INV_MOD_R.bv = 10079#32 := by simp [global_simps]
-
 
 /-!
 # Addition modulo
@@ -301,37 +260,7 @@ theorem mont_mul_twiddle_spec (k : Usize) (c : U32) (twiddleFactor : U32) (twidd
   ring_nf
   fsimp [Spec.ζ]
 
-def wfArray {n} (a : Array U16 n) : Prop :=
-  ∀ i, i < n.val → a.val[i]!.val < 3329
-
-@[local progress]
-theorem wfArray_update {n : Usize} (v : Std.Array U16 n) (i : Usize) (x : U16)
-  (hbound : i.val < v.length)
-  (hx : x.val < 3329)
-  (hWf : wfArray v) :
-  ∃ nv, v.update i x = ok nv ∧ nv = v.set i x ∧
-  wfArray nv := by
-  progress as ⟨ nv, hnv ⟩
-  fsimp [wfArray] at *
-  fsimp [hnv, toResult]
-  intro j hj
-  dcases hLt : j = i.val <;> fsimp [*]
-
-@[local progress]
-theorem wfArray_index {n : Usize} (v : Std.Array U16 n) (i : Usize)
-  (hbound : i.val < v.length)
-  (hWf : wfArray v) :
-  ∃ x, v.index_usize i = ok x ∧ x = v.val[i.val]! ∧ x.val < 3329 := by
-  progress as ⟨ x ⟩
-  fsimp [wfArray] at hWf
-  fsimp [*]
-  replace hWf := hWf i.val (by scalar_tac)
-  scalar_tac
-
-theorem wfArray_iff_forAll {n : Usize} (a : Std.Array U16 n) : wfArray a ↔ a.val.all (fun x => x.val < 3329) := by
-  simp +contextual only [wfArray, List.getElem!_eq_getElem?_getD, List.Vector.length_val,
-    List.getElem?_eq_getElem, Option.getD_some, List.all_eq_true, decide_eq_true_eq, ←
-    List.forall_getElem]
+attribute [local progress] wfArray_update wfArray_index
 
 @[simp]
 theorem wfArray_zetaTwoTimesBitRevPlus1TimesR : wfArray ZETA_TO_TIMES_BIT_REV_PLUS_1_TIMES_R := by
