proofs/Symcrust/Properties/Basic.lean
@@ -1,0 +1,88 @@
+import Symcrust.Properties.Polynomials
+import Symcrust.Code.Funs
+
+#setup_aeneas_simps
+
+namespace Symcrust
+
+open Aeneas Aeneas.Std Result
+
+namespace ntt
+
+def to_poly (a : Array U16 256#usize) : Spec.Polynomial := Vector.ofFn (fun i => a[i]!)
+
+@[simp]
+theorem getElem!_to_poly (a : Array U16 256#usize) (i : ℕ) :
+  (to_poly a)[i]! = ((a.val[i]!) : Spec.Zq) := by
+  simp [to_poly]
+  dcases hi : i < a.val.length <;> simp_all [default, Vector.getElem!_ofFn]
+
+@[simp]
+theorem to_poly_set (a : Array U16 256#usize) (i : Usize) (x : U16) :
+  to_poly (Std.Array.set a i x) = (to_poly a).set! i.val (x.val : Spec.Zq) := by
+  simp only [to_poly, Spec.Q, id_eq, Array.set_val_eq, List.map_set]
+  rw [Vector.eq_iff_forall_eq_getElem!]
+  intro j hj
+  simp_lists
+  by_cases hj': j = i <;> simp only [Fin.getElem!_fin, Array.getElem!_Nat_eq, Array.set_val_eq,
+    Nat.not_eq, ne_eq, not_false_eq_true, lt_or_lt_iff_ne, true_or, or_true, List.getElem!_set_ne,
+    id_eq, hj']
+  simp_lists
+  simp_lists -- TODO: why do we need two calls?
+
+@[simp]
+theorem to_poly_getElem!_eq (a : Std.Array U16 256#usize) (i : Nat) :
+  (to_poly a)[i]! = a.val[i]! := by
+  fsimp [to_poly]
+  dcases h: i < 256 <;> simp_all [Vector.getElem!_ofFn, default]
+
+-- TODO: move all
+
+def wfArray {n} (a : Array U16 n) : Prop :=
+  ∀ i, i < n.val → a.val[i]!.val < 3329
+
+theorem wfArray_update {n : Usize} (v : Std.Array U16 n) (i : Usize) (x : U16)
+  (hbound : i.val < v.length)
+  (hx : x.val < 3329)
+  (hWf : wfArray v) :
+  ∃ nv, v.update i x = ok nv ∧ nv = v.set i x ∧
+  wfArray nv := by
+  progress as ⟨ nv, hnv ⟩
+  fsimp [wfArray] at *
+  fsimp [hnv, toResult]
+  intro j hj
+  dcases hLt : j = i.val <;> fsimp [*]
+
+theorem wfArray_index {n : Usize} (v : Std.Array U16 n) (i : Usize)
+  (hbound : i.val < v.length)
+  (hWf : wfArray v) :
+  ∃ x, v.index_usize i = ok x ∧ x = v.val[i.val]! ∧ x.val < 3329 := by
+  progress as ⟨ x ⟩
+  fsimp [wfArray] at hWf
+  fsimp [*]
+  replace hWf := hWf i.val (by scalar_tac)
+  scalar_tac
+
+theorem wfArray_iff_forAll {n : Usize} (a : Std.Array U16 n) : wfArray a ↔ a.val.all (fun x => x.val < 3329) := by
+  simp +contextual only [wfArray, List.getElem!_eq_getElem?_getD, List.Vector.length_val,
+    List.getElem?_eq_getElem, Option.getD_some, List.all_eq_true, decide_eq_true_eq, ←
+    List.forall_getElem]
+
+@[simp, scalar_tac_simps, bvify_simps] theorem Q.eq : Q = 3329#u32 := by simp [global_simps]
+@[simp, scalar_tac_simps, bvify_simps] theorem NEG_Q_INV_MOD_R.eq : NEG_Q_INV_MOD_R = 3327#u32 := by simp [global_simps]
+@[simp, scalar_tac_simps, bvify_simps] theorem RMASK.eq : RMASK = 65535#u32 := by simp [global_simps]
+@[simp, scalar_tac_simps, bvify_simps] theorem RLOG2.eq : RLOG2 = 16#u32 := by simp [global_simps]
+@[simp, scalar_tac_simps, bvify_simps] theorem RSQR.eq : RSQR = 1353#u32 := by simp [global_simps]
+@[simp, scalar_tac_simps, bvify_simps] theorem RSQR_TIMES_NEG_Q_INV_MOD_R.eq : RSQR_TIMES_NEG_Q_INV_MOD_R = 44983#u32 := by simp [global_simps]
+
+@[simp, scalar_tac_simps, bvify_simps]
+theorem key.MLWE_POLYNOMIAL_COEFFICIENTS_eq : key.MLWE_POLYNOMIAL_COEFFICIENTS.val = 256 := by simp [global_simps]
+
+@[simp] theorem INTT_FIXUP_TIMES_RSQR.eq : INTT_FIXUP_TIMES_RSQR.val = 1441 := by simp [global_simps]
+@[simp] theorem INTT_FIXUP_TIMES_RSQR.bv_eq : INTT_FIXUP_TIMES_RSQR.bv = 1441#32 := by simp [global_simps]
+
+@[simp] theorem INTT_FIXUP_TIMES_RSQR_TIMES_NEQ_Q_INV_MOD_R.bv_eq : INTT_FIXUP_TIMES_RSQR_TIMES_NEQ_Q_INV_MOD_R.bv = 10079#32 := by simp [global_simps]
+
+end ntt
+
+end Symcrust
